theories/SLFHprop.v
@@ -14,9 +14,9 @@ License: MIT.
 
 Set Implicit Arguments.
 From Sep Require Export SLFExtra.
+Import SLFProgramSyntax.
 
-(** Configuration of Fmap.v *)
-
+(** Tweak to simplify the use of definitions and lemmas from [Fmap.v]. *)
 Arguments Fmap.single {A} {B}.
 Arguments Fmap.union {A} {B}.
 Arguments Fmap.disjoint {A} {B}.
@@ -27,11 +27,15 @@ Arguments Fmap.union_assoc {A} {B}.
 Arguments Fmap.disjoint_union_eq_l {A} {B}.
 Arguments Fmap.disjoint_union_eq_r {A} {B}.
 
+(** Tweak to enable the parsing of concrete programs in the toy language
+    defined by [SLFDirect]. *)
+(*
 Local Close Scope fmap_scope.
 Local Open Scope string_scope.
 Local Open Scope val_scope.
 Local Open Scope trm_scope.
 Local Coercion string_to_var (x:string) : var := x.
+*)
 
 
 (* ########################################################### *)
